00Utils/Iteration.thy
@@ -4,8 +4,8 @@ begin
 
 subsection \<open>Reflexive Transitive Closure\<close>
 
-text \<open>We define the reflexive transitive closure of a relation. This will be used for iterating 
-evaluation steps.\<close>
+text \<open>Our final utility is the reflexive transitive closure of a relation. This will be used for 
+iterating evaluation steps.\<close>
 
 inductive iter :: "('a \<Rightarrow> 'a \<Rightarrow> bool) \<Rightarrow> 'a \<Rightarrow> 'a \<Rightarrow> bool" for f where
   iter_refl [simp]: "iter f a a"
